Cslib/Computability/Machines/MultiTapeTuring/Routines/Typed.lean
@@ -27,7 +27,7 @@ public def computes_function_update {k : ℕ}
 public def computes_function_read_update {k : ℕ}
   {α : Type} [StrEnc α]
   (tm : MultiTapeTM k Char) (f : α → TapeView → TapeView)
-  (i j : Fin k) (_h_neq : i ≠ j) :=
+  (i j : Fin k) :=
   ∀ (x : α) (views : Fin k → TapeView),
     ((views i).current = StrEnc.toData x) →
     tm.eval_struct views = .some (Function.update views j (f x (views j)))
@@ -36,7 +36,7 @@ public def computes_function_read_update {k : ℕ}
 public def computes_function_read_update' {k : ℕ}
   {α β : Type} [StrEnc α] [StrEnc β]
   (tm : MultiTapeTM k Char) (f : α → β → β)
-  (i j : Fin k) (_h_neq : i ≠ j) :=
+  (i j : Fin k) :=
   ∀ (x : α) (y : β) (views : Fin k → TapeView),
     ((views i).current = StrEnc.toData x) →
     views j = TapeView.ofEnc y →
@@ -46,7 +46,7 @@ public def computes_function_read_update' {k : ℕ}
 public def computes_function_read_read_update {k : ℕ}
   {α β : Type} [StrEnc α] [StrEnc β]
   (tm : MultiTapeTM k Char) (f : α → β → TapeView → TapeView)
-  (i j r : Fin k) (_h_neq : [i, j, r].get.Injective) :=
+  (i j r : Fin k) :=
   ∀ (x : α) (y : β) (views : Fin k → TapeView),
     ((views i).current = StrEnc.toData x) →
     ((views j).current = StrEnc.toData y) →
@@ -56,7 +56,7 @@ public def computes_function_read_read_update {k : ℕ}
 public def computes_function_read_read_update' {k : ℕ}
   {α β γ : Type} [StrEnc α] [StrEnc β] [StrEnc γ]
   (tm : MultiTapeTM k Char) (f : α → β → γ → γ)
-  (i j r : Fin k) (_h_neq : [i, j, r].get.Injective) :=
+  (i j r : Fin k) :=
   ∀ (x : α) (y : β) (z : γ) (views : Fin k → TapeView),
     ((views i).current = StrEnc.toData x) →
     ((views j).current = StrEnc.toData y) →
@@ -71,16 +71,16 @@ public def computes_function_read_read_update' {k : ℕ}
 --   {α β : Type} [StrEnc α] [StrEnc β]
 --   (tm : MultiTapeTM k Char)
 --   (f : α → β)
---   (i j : Fin k) (h_neq : i ≠ j) :=
---   computes_function_read_update tm (fun d tv => tv.pushList (StrEnc.toData (f d))) i j h_neq
+--   (i j : Fin k) :=
+--   computes_function_read_update tm (fun d tv => tv.pushList (StrEnc.toData (f d))) i j
 
 @[expose]
 public def computes_function_read_push {k : ℕ}
   {α β : Type} [StrEnc α] [StrEnc β]
   (tm : MultiTapeTM k Char)
   (f : α → β)
-  (i j : Fin k) (h_neq : i ≠ j) :=
-  computes_function_read_update tm (fun d tv => tv.pushList (StrEnc.toData (f d))) i j h_neq
+  (i j : Fin k) :=
+  computes_function_read_update tm (fun d tv => tv.pushList (StrEnc.toData (f d))) i j
 
 -- If the list is heterogeneous, use β = Data
 @[expose]
@@ -88,26 +88,26 @@ public def computes_function_read_push' {k : ℕ}
   {α β : Type} [StrEnc α] [StrEnc β]
   (tm : MultiTapeTM k Char)
   (f : α → β)
-  (i j : Fin k) (h_neq : i ≠ j) :=
-  computes_function_read_update' tm (fun d ls => (f d) :: ls) i j h_neq
+  (i j : Fin k) :=
+  computes_function_read_update' tm (fun d ls => (f d) :: ls) i j
 
 @[expose]
 public def computes_function_read_read_push {k : ℕ}
   {α β γ : Type} [StrEnc α] [StrEnc β] [StrEnc γ]
   (tm : MultiTapeTM k Char)
   (f : α → β → γ)
-  (i j s : Fin k) (h_neq : [i, j, s].get.Injective) :=
+  (i j s : Fin k) :=
   computes_function_read_read_update tm
-    (fun x y tv => tv.pushList (StrEnc.toData (f x y))) i j s h_neq
+    (fun x y tv => tv.pushList (StrEnc.toData (f x y))) i j s
 
 @[expose]
 public def computes_function_read_read_push' {k : ℕ}
   {α β γ : Type} [StrEnc α] [StrEnc β] [StrEnc γ]
   (tm : MultiTapeTM k Char)
   (f : α → β → γ)
-  (i j s : Fin k) (h_neq : [i, j, s].get.Injective) :=
+  (i j s : Fin k) :=
   computes_function_read_read_update' tm
-    (fun x y (ls : List Data) => StrEnc.toData (f x y) :: ls) i j s h_neq
+    (fun x y (ls : List Data) => StrEnc.toData (f x y) :: ls) i j s
 
 
 /-- Turing machine `tm` updates the head of tape `i`. -/
@@ -122,74 +122,28 @@ public def computes_function_head_update {k : ℕ}
 public theorem computes_function_seq₁ {k : ℕ}
   {α β γ : Type} [StrEnc α] [StrEnc β] [StrEnc γ]
   {tm₁ tm₂ : MultiTapeTM k Char} {f₁ : α → β} {f₂ : β → γ}
-  {i j : Fin k} (h_neq : i ≠ j)
-  (h_comp₁ : computes_function_read_push tm₁ f₁ i j h_neq)
+  {i j : Fin k}
+  (h_comp₁ : computes_function_read_push tm₁ f₁ i j)
   (h_comp₂ : computes_function_head_update tm₂ f₂ j) :
-  computes_function_read_push (tm₁ ;ₜ tm₂) (fun x => f₂ (f₁ x)) i j h_neq := by sorry
+  computes_function_read_push (tm₁ ;ₜ tm₂) (fun x => f₂ (f₁ x)) i j := by sorry
 
 @[simp, grind =>]
 public theorem computes_function_seq₂ {k : ℕ}
   {α β γ δ : Type} [StrEnc α] [StrEnc β] [StrEnc γ] [StrEnc δ]
   {tm₁ tm₂ : MultiTapeTM k Char} {f₁ : α → β → γ} {f₂ : γ → δ}
-  {i j r : Fin k} (h_neq : [i, j, r].get.Injective)
-  (h_comp₁ : computes_function_read_read_push tm₁ f₁ i j r h_neq)
+  {i j r : Fin k}
+  (h_comp₁ : computes_function_read_read_push tm₁ f₁ i j r)
   (h_comp₂ : computes_function_head_update tm₂ f₂ r) :
-  computes_function_read_read_push (tm₁ ;ₜ tm₂) (fun x y => f₂ (f₁ x y)) i j r h_neq := by sorry
+  computes_function_read_read_push (tm₁ ;ₜ tm₂) (fun x y => f₂ (f₁ x y)) i j r := by sorry
 
 
 @[grind =>]
 public theorem computes_function_read_read_push_swap {k : ℕ}
   {α β γ : Type} [StrEnc α] [StrEnc β] [StrEnc γ]
   {tm : MultiTapeTM k Char} {f : α → β → γ}
-  {i j r : Fin k} {h_neq : [i, j, r].get.Injective}
-  (h : computes_function_read_read_push tm f i j r h_neq) :
-  computes_function_read_read_push tm (fun x y => f y x) j i r
-    (by sorry) := by sorry
-
-inductive TapeEffects where
-  | read
-  | consume
-  | put
-  | modify
-
--- and all indices different
-def FunArgs (k : ℕ) := List ((Fin k) × TapeEffects)
-
-def ReturnType {k : ℕ} (args : FunArgs k) : Type := match args with
- | [] => Unit
- | (_, .read) :: rest => ReturnType rest
- | (_, .consume) :: rest => ReturnType rest
- | (_, .put) :: rest => Data × ReturnType rest
- | (_, .modify) :: rest => Data × ReturnType rest
-
-def InputTypes {k : ℕ} (args : FunArgs k) : Type := match args with
- | [] => Unit
- | (_, .read) :: rest => Data → (InputTypes rest)
- | (_, .consume) :: rest => Data → (InputTypes rest)
- | (_, .put) :: rest => InputTypes rest
- | (_, .modify) :: rest => Data → (InputTypes rest)
-
-def TypeOfFunArgs {k : ℕ} (args : FunArgs k) : Type := (InputTypes args) → (ReturnType args)
-
--- def EvaluateFun {k : ℕ} (args : FunArgs k) (views : Fin k → TapeView)
---   (f : TypeOfFunArgs args) : Option (ReturnType args) := match args with
---   | [] => some ()
---   | (i, .read) :: rest => (views i).current.bind (fun d => EvaluateFun rest views (f d))
---   | (_, .consume) :: rest => Data → (InputTypes rest)
---   | (_, .put) :: rest => InputTypes rest
---   | (_, .modify) :: rest => Data → (InputTypes rest)
-
---   --(i, TapeEffects.read) :: rest =>
---     let current := (views i).current
---     current.bind (fun d => EvaluateFun rest views (f d))
-
--- public def computes_function_general {k : ℕ}
---   (tm : MultiTapeTM k Char) (f : TapeView → Data → TapeView)
---   (i j : Fin k) (_h_neq : i ≠ j)
---   (views : Fin k → TapeView) :=
---   tm.eval_struct views = some (Function.update views j
---     (((views i).current.map (f (views j))).getD (views j)))
-
+  {i j r : Fin k}
+  (h : computes_function_read_read_push tm f i j r) :
+  computes_function_read_read_push tm (fun x y => f y x) j i r := by sorry
 
 
 end Routines
