Cslib/Computability/Machines/MultiTapeTuring/Routines/MultiTape.lean
@@ -38,7 +38,7 @@ public lemma isEq.computes_fun {k : ℕ} (i j result : Fin k)
     (h_neq : [i, j, result].get.Injective) :
     computes_function_read_read_push
       (isEq i j result)
-      (fun (d₁ : α) (d₂ : α) => d₂ == d₁) i j result h_neq := by
+      (fun (d₁ : α) (d₂ : α) => d₂ == d₁) i j result := by
   sorry
 
 /-- `copyEnc i j` copies the `Data` element at the current path position
